SStructTT/SStruct/Runtime/Step.lean
@@ -6,8 +6,9 @@ namespace Runtime
 
 variable {Srt : Type} [ord : SrtOrder Srt]
 
+/- Deallocate dropped terms. -/
 inductive Drop : Heap Srt -> Tm Srt -> Heap Srt -> Prop where
-  | var {H x} : Drop H x H
+  | var {H x} : Drop H (.var x) H
   | lam {H1 H2 m s} :
     Drop H1 m H2 ->
     Drop H1 (.lam m s) H2
@@ -40,11 +41,27 @@ inductive Drop : Heap Srt -> Tm Srt -> Heap Srt -> Prop where
     Drop H1 (.ptr l) H3
   | null {H} : Drop H .null H -- free(NULL) in C does nothing
 
+/- Force drop-reductions to have deterministic eval order.  -/
+@[simp]def DropFree : Tm Srt -> Prop
+  | .var _ => True
+  | .lam _ _ => True
+  | .app m n => DropFree m ∧ DropFree n
+  | .tup m n _ => DropFree m ∧ DropFree n
+  | .prj m _ => DropFree m
+  | .tt => True
+  | .ff => True
+  | .ite m _ _ => DropFree m
+  | .drop _ _ => False
+  | .ptr _ => True
+  | .null => True
+
+/- Possibly NULL pointers. -/
 @[scoped aesop safe [constructors]]
 inductive Nullptr : Tm Srt -> Prop where
   | ptr {l} : Nullptr (.ptr l)
   | null    : Nullptr .null
 
+/- Heap allocated values. -/
 @[scoped aesop safe [constructors]]
 inductive HValue : Tm Srt -> Srt -> Prop where
   | lam {m s}   : HValue (.lam m s) s
@@ -52,75 +69,321 @@ inductive HValue : Tm Srt -> Srt -> Prop where
   | tt : HValue .tt ord.e
   | ff : HValue .ff ord.e
 
+/- State (Heap + Term) of the evaluator. -/
 abbrev State Srt := Heap Srt × Tm Srt
 
+/- Drop-reductions. -/
 @[scoped aesop safe [constructors]]
 inductive Step0 : State Srt -> State Srt -> Prop where
   | app_M {H1 H2 m m'} n :
     Step0 (H1, m) (H2, m') ->
     Step0 (H1, .app m n) (H2, .app m' n)
   | app_N {H1 H2} m {n n'} :
+    DropFree m ->
     Step0 (H1, n) (H2, n') ->
     Step0 (H1, .app m n) (H2, .app m n')
   | tup_M {H1 H2 m m'} n s :
     Step0 (H1, m) (H2, m') ->
-    Step0 (H2, .tup m n s) (H2, .tup m' n s)
+    Step0 (H1, .tup m n s) (H2, .tup m' n s)
   | tup_N {H1 H2} m {n n'} s :
+    DropFree m ->
     Step0 (H1, n) (H2, n') ->
-    Step0 (H2, .tup m n s) (H2, .tup m n' s)
+    Step0 (H1, .tup m n s) (H2, .tup m n' s)
   | prj_M {H1 H2 m m'} n :
     Step0 (H1, m) (H2, m') ->
     Step0 (H1, .prj m n) (H2, .prj m' n)
   | ite_M {H1 H2 m m'} n1 n2 :
     Step0 (H1, m) (H2, m') ->
     Step0 (H1, .ite m n1 n2) (H2, .ite m' n1 n2)
-  | alloc {H v s l} :
-    l ∉ H.keys ->
-    HValue v s ->
-    Step0 (H, v) (H.insert l ⟨v, s⟩, .ptr l)
   | drop_elim {H1 H2 m n} :
     Drop H1 m H2 ->
     Step0 (H1, .drop m n) (H2, n)
 
+/- Alloc-reductions. -/
 @[scoped aesop safe [constructors]]
 inductive Step1 : State Srt -> State Srt -> Prop where
+  | app_M {H1 H2 m m'} n :
+    Step1 (H1, m) (H2, m') ->
+    Step1 (H1, .app m n) (H2, .app m' n)
+  | app_N {H1 H2} l {n n'} :
+    Step1 (H1, n) (H2, n') ->
+    Step1 (H1, .app (.ptr l) n) (H2, .app (.ptr l) n')
+  | tup_M {H1 H2 m m'} n s :
+    Step1 (H1, m) (H2, m') ->
+    Step1 (H2, .tup m n s) (H2, .tup m' n s)
+  | tup_N {H1 H2} l {n n'} s :
+    Step1 (H1, n) (H2, n') ->
+    Step1 (H2, .tup (.ptr l) n s) (H2, .tup (.ptr l) n' s)
+  | prj_M {H1 H2 m m'} n :
+    Step1 (H1, m) (H2, m') ->
+    Step1 (H1, .prj m n) (H2, .prj m' n)
+  | ite_M {H1 H2 m m'} n1 n2 :
+    Step1 (H1, m) (H2, m') ->
+    Step1 (H1, .ite m n1 n2) (H2, .ite m' n1 n2)
+  | alloc {H v s l} :
+    l ∉ H.keys ->
+    HValue v s ->
+    Step1 (H, v) (H.insert l ⟨v, s⟩, .ptr l)
+
+/- Core-reductions. -/
+@[scoped aesop safe [constructors]]
+inductive Step2 : State Srt -> State Srt -> Prop where
   | app_M {H H' m m' n} :
-    Step1 (H, m) (H', m') ->
-    Step1 (H, .app m n) (H', .app m' n)
+    Step2 (H, m) (H', m') ->
+    Step2 (H, .app m n) (H', .app m' n)
   | app_N {H H' m n n'} :
-    Step1 (H, n) (H', n') ->
-    Step1 (H, .app m n) (H', .app m n')
+    Step2 (H, n) (H', n') ->
+    Step2 (H, .app m n) (H', .app m n')
   | beta {H1 H2 m s lf p} :
     Nullptr p ->
     HLookup H1 lf (.lam m s) H2 ->
-    Step1 (H1, .app (.ptr lf) p) (H2, m.[p/])
+    Step2 (H1, .app (.ptr lf) p) (H2, m.[p/])
   | tup_M {H H' m m' n s} :
-    Step1 (H, m) (H', m') ->
-    Step1 (H, .tup m n s) (H', .tup m' n s)
+    Step2 (H, m) (H', m') ->
+    Step2 (H, .tup m n s) (H', .tup m' n s)
   | tup_N {H H' m n n' s} :
-    Step1 (H, n) (H', n') ->
-    Step1 (H, .tup m n s) (H', .tup m n' s)
+    Step2 (H, n) (H', n') ->
+    Step2 (H, .tup m n s) (H', .tup m n' s)
   | prj_M {H H' m m' n} :
-    Step1 (H, m) (H', m') ->
-    Step1 (H, .prj m n) (H', .prj m' n)
+    Step2 (H, m) (H', m') ->
+    Step2 (H, .prj m n) (H', .prj m' n)
   | prj_elim {H1 H2 H3 n s l l1 p} :
     Nullptr p ->
     HLookup H1 l (.tup (.ptr l1) p s) H2 ->
-    Step1 (H1, .prj (.ptr l) n) (H3, n.[p,.ptr l1/])
+    Step2 (H1, .prj (.ptr l) n) (H3, n.[p,.ptr l1/])
   | ite_M {H H' m m' n1 n2} :
-    Step1 (H, m) (H', m') ->
-    Step1 (H, .ite m n1 n2) (H', .ite m' n1 n2)
+    Step2 (H, m) (H', m') ->
+    Step2 (H, .ite m n1 n2) (H', .ite m' n1 n2)
   | ite_tt {H H' n1 n2 l} :
     HLookup H l .tt H' ->
-    Step1 (H, .ite (.ptr l) n1 n2) (H', n1)
+    Step2 (H, .ite (.ptr l) n1 n2) (H', n1)
   | ite_ff {H H' n1 n2 l} :
     HLookup H l .ff H' ->
-    Step1 (H, .ite (.ptr l) n1 n2) (H', n2)
+    Step2 (H, .ite (.ptr l) n1 n2) (H', n2)
 
 abbrev Red0 (t1 t2 : @State Srt) : Prop := Star Step0 t1 t2
+abbrev Red1 (t1 t2 : @State Srt) : Prop := Star Step1 t1 t2
 
 inductive Step (m : State Srt) : State Srt -> Prop where
-  | intro {m' n} : Red0 m m' -> Step1 m' n -> Step m n
+  | intro {x y n} : Red0 m x -> Red1 x y -> Step2 y n -> Step m n
 
-notation:50 H:50 " ;; " m:51 " ~>> " H':51 " ;; " m':51 =>
-  Step (H, m) (H', m')
+notation:50 t:50 " ~>> " t':51 => Step t t'
+notation:50 t:50 " ~>>* " t':51 => Star Step t t'
+
+lemma Step0.not_dropfree {H m} {t : State Srt} :
+    Step0 (H, m) t -> ¬ DropFree m := by
+  generalize e: (H, m) = t0
+  intro st; induction st generalizing H m
+  all_goals cases e; aesop
+
+lemma Red0.var_inv {H x} {t : State Srt} :
+    Red0 (H, .var x) t -> t = (H, .var x) := by
+  intro rd; induction rd
+  case R => simp
+  case SE st ih =>
+    subst_vars; cases st
+
+lemma Red0.lam_inv {H m s} {t : State Srt}  :
+    Red0 (H, .lam m s) t -> t = (H, .lam m s) := by
+  intro rd; induction rd
+  case R => simp
+  case SE st e => subst_vars; cases st
+
+lemma Red0.app_inv' {H1 m n} {t : State Srt} :
+    Red0 (H1, .app m n) t ->
+    ∃ H2 H3 m' n',
+      t = (H3, .app m' n') ∧
+      Red0 (H1, m) (H2, m') ∧
+      Red0 (H2, n) (H3, n') ∧
+      (¬DropFree m' -> H2 = H3 ∧ n = n') := by
+  intro rd; induction rd
+  case R =>
+    exists H1, H1, m, n; aesop
+  case SE st ih =>
+    rcases ih with ⟨H2, H3, m', n', e, rd1, rd2, h⟩
+    subst_vars
+    cases st
+    case app_M Hx mx st =>
+      have ⟨e1, e2⟩ := h st.not_dropfree; subst_vars
+      exists Hx, Hx, mx, n'; simp; and_intros
+      apply Star.SE rd1 st
+      apply Star.R
+    case app_N Hx nx h st =>
+      exists H2, Hx, m', nx; simp; and_intros
+      . assumption
+      . apply Star.SE rd2 st
+      . intro; contradiction
+
+lemma Red0.app_inv {H1 m n} {t : State Srt} :
+    Red0 (H1, .app m n) t ->
+    ∃ H2 H3 m' n',
+      t = (H3, .app m' n') ∧
+      Red0 (H1, m) (H2, m') ∧
+      Red0 (H2, n) (H3, n') := by
+  intro rd; have := rd.app_inv'; aesop
+
+lemma Red0.tup_inv' {H1 m n s} {t : State Srt} :
+    Red0 (H1, .tup m n s) t ->
+    ∃ H2 H3 m' n',
+      t = (H3, .tup m' n' s) ∧
+      Red0 (H1, m) (H2, m') ∧
+      Red0 (H2, n) (H3, n') ∧
+      (¬DropFree m' -> H2 = H3 ∧ n = n') := by
+  intro rd; induction rd
+  case R =>
+    exists H1, H1, m, n; aesop
+  case SE st ih =>
+    rcases ih with ⟨H2, H3, m', n', e, rd1, rd2, h⟩
+    subst_vars
+    cases st
+    case tup_M Hx mx st =>
+      have ⟨e1, e2⟩ := h st.not_dropfree; subst_vars
+      exists Hx, Hx, mx, n'; simp; and_intros
+      apply Star.SE rd1 st
+      apply Star.R
+    case tup_N Hx nx h st =>
+      exists H2, Hx, m', nx; simp; and_intros
+      . assumption
+      . apply Star.SE rd2 st
+      . intro; contradiction
+
+lemma Red0.tup_inv {H1 m n s} {t : State Srt} :
+    Red0 (H1, .tup m n s) t ->
+    ∃ H2 H3 m' n',
+      t = (H3, .tup m' n' s) ∧
+      Red0 (H1, m) (H2, m') ∧
+      Red0 (H2, n) (H3, n') := by
+  intro rd; have := rd.tup_inv'; aesop
+
+lemma Red0.prj_inv {H1 m n} {t : State Srt} :
+    Red0 (H1, .prj m n) t ->
+    ∃ H2 m', t = (H2, .prj m' n) ∧ Red0 (H1, m) (H2, m') := by
+  intro rd; induction rd
+  case R => exists H1, m; aesop
+  case SE st ih =>
+    rcases ih with ⟨H2, m', e, rd⟩
+    subst_vars; cases st
+    case prj_M Hx mx st =>
+      exists Hx, mx; simp
+      apply Star.SE rd st
+
+lemma Red0.tt_inv {H1} (t : State Srt) :
+    Red0 (H1, .tt) t -> t = (H1, .tt) := by
+  intro rd; induction rd
+  case R => simp
+  case SE st e => subst_vars; cases st
+
+lemma Red0.ff_inv {H1} (t : State Srt) :
+    Red0 (H1, .ff) t -> t = (H1, .ff) := by
+  intro rd; induction rd
+  case R => simp
+  case SE st e => subst_vars; cases st
+
+lemma Red0.ite_inv {H1 m n1 n2} {t : State Srt} :
+    Red0 (H1, .ite m n1 n2) t ->
+    ∃ H2 m', t = (H2, .ite m' n1 n2) ∧ Red0 (H1, m) (H2, m') := by
+  intro rd; induction rd
+  case R => simp; aesop
+  case SE rd st ih =>
+    rcases ih with ⟨H2, m', e, rd0⟩
+    subst_vars; cases st
+    case ite_M Hx mx st =>
+      exists Hx, mx; simp
+      apply Star.SE rd0 st
+
+lemma Red0.ptr_inv {H1 l} {t : State Srt} :
+    Red0 (H1, .ptr l) t -> t = (H1, .ptr l) := by
+  intro rd; induction rd
+  case R => simp
+  case SE st e => subst_vars; cases st
+
+lemma Red0.null_inv {H1} {t : State Srt} :
+    Red0 (H1, .null) t -> t = (H1, .null) := by
+  intro rd; induction rd
+  case R => simp
+  case SE st e => subst_vars; cases st
+
+lemma Red0.app_M {H1 H2} {m m' n : Tm Srt} :
+    Red0 (H1, m) (H2, m') ->
+    Red0 (H1, .app m n) (H2, .app m' n) := by
+  intro rm
+  apply Star.hom (fun (H, x) => (H, Tm.app x n)) _ rm (e2 := Step0)
+  simp; aesop
+
+lemma Drop.wr_image {H1 H2 : Heap Srt} {m} :
+    Drop H1 m H2 -> WR H1 -> WR H2 := by
+  intro dp wr; induction dp
+  all_goals try (solve|aesop)
+  case ptr lk dp ih => have := lk.wr_image wr; aesop
+
+lemma Drop.resolve {H1 H2 H3 H3' : Heap Srt} {m m' s} :
+    HMerge H1 H2 H3 -> HLower H1 s -> s ∈ ord.weaken_set ->
+    H1 ⊢ m ▷ m' -> Drop H3 m H3' ->
+    ∃ H1', HMerge H1' H2 H3' ∧ HLower H1' ord.e := by
+  intro mrg0 lw0 h0 rs0 dp0; induction rs0 generalizing H2 H3 H3' s
+  case var H x lw => cases dp0; exists H
+  case lam => cases dp0; aesop
+  case app mrg rsm rsn ihm ihn =>
+    cases dp0; case app dp1 dp2 =>
+    have ⟨H1x, mrg1, mrg2⟩ := mrg0.split mrg.sym
+    have ⟨lw1, lw2⟩ := mrg.split_lower lw0
+    have ⟨H2x, mrg3, lw3⟩ := ihm mrg2.sym lw1 h0 dp1
+    have ⟨H3x, mrg4, mrg5⟩ := mrg3.sym.split mrg1.sym
+    have ⟨H4x, mrg6, lw4⟩ := ihn mrg5.sym lw2 h0 dp2
+    have ⟨H5x, mrg7, mrg8⟩ := mrg6.sym.split mrg4.sym
+    exists H5x; and_intros
+    . assumption
+    . apply mrg7.lower_image lw3 lw4
+  case tup mrg rsm rsn ihm ihn =>
+    cases dp0; case tup dp1 dp2 =>
+    have ⟨H1x, mrg1, mrg2⟩ := mrg0.split mrg.sym
+    have ⟨lw1, lw2⟩ := mrg.split_lower lw0
+    have ⟨H2x, mrg3, lw3⟩ := ihm mrg2.sym lw1 h0 dp1
+    have ⟨H3x, mrg4, mrg5⟩ := mrg3.sym.split mrg1.sym
+    have ⟨H4x, mrg6, lw4⟩ := ihn mrg5.sym lw2 h0 dp2
+    have ⟨H5x, mrg7, mrg8⟩ := mrg6.sym.split mrg4.sym
+    exists H5x; and_intros
+    . assumption
+    . apply mrg7.lower_image lw3 lw4
+  case prj mrg rsm rsn ihm ihn =>
+    cases dp0; case prj dp1 dp2 =>
+    have ⟨H1x, mrg1, mrg2⟩ := mrg0.split mrg.sym
+    have ⟨lw1, lw2⟩ := mrg.split_lower lw0
+    have ⟨H2x, mrg3, lw3⟩ := ihm mrg2.sym lw1 h0 dp1
+    have ⟨H3x, mrg4, mrg5⟩ := mrg3.sym.split mrg1.sym
+    have ⟨H4x, mrg6, lw4⟩ := ihn mrg5.sym lw2 h0 dp2
+    have ⟨H5x, mrg7, mrg8⟩ := mrg6.sym.split mrg4.sym
+    exists H5x; and_intros
+    . assumption
+    . apply mrg7.lower_image lw3 lw4
+  case tt H1 _ => cases dp0; exists H1
+  case ff H1 _ => cases dp0; exists H1
+  case ite mrg rsm1 rsn1 rsn2 ihm ihn1 ihn2 =>
+    cases dp0; case ite dp1 dp2 dp3 =>
+    have ⟨H1x, mrg1, mrg2⟩ := mrg0.split mrg.sym
+    have ⟨lw1, lw2⟩ := mrg.split_lower lw0
+    have ⟨H2x, mrg3, lw3⟩ := ihm mrg2.sym lw1 h0 dp1
+    have ⟨H3x, mrg4, mrg5⟩ := mrg3.sym.split mrg1.sym
+    have ⟨H4x, mrg6, lw4⟩ := ihn1 mrg5.sym lw2 h0 dp2
+    have ⟨H5x, mrg7, mrg8⟩ := mrg6.sym.split mrg4.sym
+    have ⟨H4x, mrg6, lw4⟩ := ihn2 mrg5.sym lw2 h0 dp3
+    have ⟨H5x, mrg7, mrg8⟩ := mrg6.sym.split mrg4.sym
+    exists H5x; and_intros
+    . assumption
+    . apply mrg7.lower_image lw3 lw4
+  case drop mrg _ _ rsm rsn ihm ihn =>
+    cases dp0; case drop dp1 dp2 =>
+    have ⟨H1x, mrg1, mrg2⟩ := mrg0.split mrg.sym
+    have ⟨lw1, lw2⟩ := mrg.split_lower lw0
+    have ⟨H2x, mrg3, lw3⟩ := ihm mrg2.sym lw1 h0 dp1
+    have ⟨H3x, mrg4, mrg5⟩ := mrg3.sym.split mrg1.sym
+    have ⟨H4x, mrg6, lw4⟩ := ihn mrg5.sym lw2 h0 dp2
+    have ⟨H5x, mrg7, mrg8⟩ := mrg6.sym.split mrg4.sym
+    exists H5x; and_intros
+    . assumption
+    . apply mrg7.lower_image lw3 lw4
+  case ptr lk1 rs ih =>
+    cases dp0; case ptr lk2 dp =>
+    have ⟨e, mrg1⟩ := HLookup.collision mrg0 lk2 lk1; subst e
+    have lw1 := lk1.lower lw0; aesop
+  case null H1 _ => cases dp0; exists H1
